tests/cache/dep/lakefile.lean
@@ -1,0 +1,7 @@
+import Lake
+open Lake DSL
+
+package dep
+
+lean_lib Dep where
+  globs := #[Glob.submodules `Dep]
